src/library/tactic/simplify.h
@@ -168,13 +168,15 @@ public:
    and use itself to discharge hypotheses. */
 class simplify_fn : public simplify_ext_core_fn {
 protected:
+    list<name> m_to_unfold;
     virtual optional<pair<simp_result, bool>> pre(expr const & e, optional<expr> const & parent) override;
     virtual optional<pair<simp_result, bool>> post(expr const & e, optional<expr> const & parent) override;
     virtual optional<expr> prove(expr const & e) override;
 public:
-    simplify_fn(type_context & ctx, defeq_canonizer::state & dcs, simp_lemmas const & slss,
+    simplify_fn(type_context & ctx, defeq_canonizer::state & dcs, simp_lemmas const & slss, list<name> const & to_unfold,
                 simp_config const & cfg):
-        simplify_ext_core_fn(ctx, dcs, slss, cfg) {}
+        simplify_ext_core_fn(ctx, dcs, slss, cfg),
+        m_to_unfold(to_unfold) {}
 };
 
 void initialize_simplify();
