library/init/meta/converter/interactive.lean
@@ -113,7 +113,7 @@ meta def simp (no_dflt : parse only_flag) (hs : parse opt_qexpr_list) (attr_name
               : conv unit :=
 do s ← tactic.mk_simp_set no_dflt attr_names hs ids,
    (r, lhs, rhs) ← tactic.target_lhs_rhs,
-   (new_lhs, pr) ← tactic.simplify s lhs cfg.to_simp_config r cfg.discharger,
+   (new_lhs, pr) ← tactic.simplify s [] lhs cfg.to_simp_config r cfg.discharger,
    update_lhs new_lhs pr,
    return ()
 
