tests/lean/run/1093.lean
@@ -5,4 +5,4 @@ constant le.refl (a : nat) : a ≤ a
 attribute [simp] zadd
 
 example (a : nat) : 0 + a ≤ a :=
-by do simp
+by simp
